src/Manifest_Admits.v
@@ -11,7 +11,7 @@ Definition empty_ASP_Address : ASP_Address. Admitted.
 Definition UUID : Type. Admitted.
 
 (* We need this for making proofs and knowing that yes, in fact, UUID is an inhabited type *)
-Definition default_UUID : UUID. Admitted.
+Definition default_uuid : UUID. Admitted.
 
 Global Instance Eq_Class_uuid : EqClass UUID. Admitted.
 
